Add heap lang exercises.

theories/language.v
@@ -1,12 +1,159 @@
 From iris.algebra Require Export list gmap.
-From iris.heap_lang Require Export lang notation metatheory.
+From iris.heap_lang Require Export notation proofmode metatheory.
 From iris.heap_lang.lib Require Export assert.
 
+Definition swap : val := λ: "l1" "l2",
+  let: "x" := !"l1" in
+  "l1" <- !"l2";;
+  "l2" <- "x".
+
+Lemma swap_wp `{heapG Σ} l1 l2 v1 v2 :
+  l1 ↦ v1 -∗
+  l2 ↦ v2 -∗
+  WP swap #l1 #l2 {{ v, ⌜ v = #() ⌝ ∗ l1 ↦ v2 ∗ l2 ↦ v1 }}.
+Proof.
+  iIntros "Hl1 Hl2".
+  rewrite /swap.
+  wp_pures.
+  wp_load.
+  (* wp_pures is performed implicitly, so not needed *)
+  wp_load.
+  wp_store.
+  wp_store.
+  iFrame.
+  auto.
+Qed.
+
+Definition twice : val := λ: "f" "x",
+  "f" ("f" "x").
+
+Lemma twice_wp `{heapG Σ} (Ψ : val → iProp Σ) (vf vx : val) :
+  WP vf vx {{ w, WP vf w {{ Ψ }} }} -∗
+  WP twice vf vx {{ Ψ }}.
+Proof.
+  iIntros "Hvf".
+  rewrite /twice. wp_pures.
+  wp_bind (vf vx).
+  auto.
+Qed.
+
+Definition add_two : val := λ: "x",
+  twice (λ: "y", #1 + "y") "x".
+
+Lemma add_two_wp `{heapG Σ} (x : Z) :
+  WP add_two #x {{ w, ⌜ w = #(2 + x) ⌝ }}%I.
+Proof.
+  rewrite /add_two. wp_pures.
+  iApply twice_wp. wp_pures.
+  iPureIntro. auto with f_equal lia.
+Qed.
+
+Definition add_two_ref : val := λ: "l",
+  twice (λ: <>, "l" <- #1 + !"l") #().
+
+Lemma add_two_ref_wp `{heapG Σ} l (x : Z) :
+  l ↦ #x -∗
+  WP add_two_ref #l {{ w, ⌜ w = #() ⌝ ∗ l ↦ #(2 + x) }}%I.
+Proof.
+  iIntros "Hl".
+  rewrite /add_two_ref. wp_pures.
+  iApply twice_wp.
+  wp_load. wp_store.
+  wp_load. wp_store.
+  rewrite Z.add_assoc (_ : (1 + 1) = 2) //.
+  iFrame.
+  auto.
+Qed.
+
+Definition twice_ref : val := λ: "lf" "lx",
+  !"lf" (!"lf" !"lx").
+
+Lemma twice_ref_wp `{heapG Σ} (Ψ : val → iProp Σ) lf lx (vf vx : val) :
+  lf ↦ vf -∗
+  lx ↦ vx -∗
+  WP vf vx {{ w, WP vf w {{ Ψ }} }} -∗
+  WP twice_ref #lf #lx {{ Ψ }}.
+Proof.
+  iIntros "Hlf Hlx Hvf".
+  rewrite /twice_ref. wp_pures.
+  do 2 wp_load.
+  wp_bind (vf vx).
+  iApply (wp_wand with "Hvf").
+  iIntros (w) "Hvf".
+  wp_load.
+  auto.
+Qed.
+
+Definition add_two_2 : val := λ: "x",
+  let: "lx" := ref "x" in
+  let: "lf" := ref (λ: "y", #1 + "y") in
+  twice_ref "lf" "lx".
+
+Lemma add_two_2_wp `{heapG Σ} (x : Z) :
+  WP add_two_2 #x {{ w, ⌜ w = #(2 + x) ⌝ }}%I.
+Proof.
+  rewrite /add_two_2. wp_pures.
+  wp_alloc lx as "Hlx".
+  wp_alloc lf as "Hfx".
+  wp_pures.
+  iApply (twice_ref_wp with "Hfx Hlx").
+  wp_pures.
+  iPureIntro. auto with f_equal lia.
+Qed.
+
+(** UNSAFE *)
+Definition unsafe_pure : val := λ: <>,
+  if: #true then #13 else #13 #37.
+
+Lemma unsafe_pure_wp `{heapG Σ} :
+  WP unsafe_pure #() {{ v, ⌜ v = #13 ⌝ }}%I.
+Proof.
+  rewrite /unsafe_pure.
+  wp_pures.
+  auto.
+Qed.
+
+Definition unsafe_ref : val := λ: <>,
+  let: "l" := ref #0 in "l" <- #true;; !"l".
+
+Lemma unsafe_ref_wp `{heapG Σ} :
+  WP unsafe_ref #() {{ v, ⌜ v = #true ⌝ }}%I.
+Proof.
+  rewrite /unsafe_ref. wp_pures.
+  wp_alloc l.
+  wp_store.
+  wp_load.
+  auto.
+Qed.
+
+(** Polymorphism *)
 (** We model type-level lambdas and applications as thunks since heap_lang does
 not have them. *)
 Notation "Λ: e" := (λ: <>, e)%E (at level 200, only parsing) : expr_scope.
 Notation "Λ: e" := (λ: <>, e)%V (at level 200, only parsing) : val_scope.
 Notation "e '<_>'" := (App e%E #()) (at level 10, only parsing) : expr_scope.
+
+Definition swap_poly : val := Λ: λ: "l1" "l2",
+  let: "x" := !"l1" in
+  "l1" <- !"l2";;
+  "l2" <- "x".
+
+Lemma swap_poly_wp `{heapG Σ} l1 l2 v1 v2 :
+  l1 ↦ v1 -∗
+  l2 ↦ v2 -∗
+  WP swap_poly <_> #l1 #l2 {{ v, ⌜ v = #() ⌝ ∗ l1 ↦ v2 ∗ l2 ↦ v1 }}.
+Proof.
+  iIntros "Hl1 Hl2".
+  rewrite /swap_poly.
+  wp_pures.
+  wp_load.
+  (* wp_pures is performed implicitly, so not needed *)
+  wp_load.
+  wp_store.
+  wp_store.
+  iFrame.
+  auto.
+Qed.
 
 (** We wrap unpack into an explicitly function so that we can have a nice
 notation for it. *)
